Extend bvi_tailrec analysis with type contexts
Implementation changed to allow for a slightly larger class of
expressions. Rewrites

> fun f x = ... ; f x' + y

to

> fun f x acc = ... ; f x' (y + acc)

Previously y was required to be integer constants or operations on
these. These changes should at least allow y to contain variables
so long as they are arguments to the function f.

Note: adjusting the theorems, so this commit upsets the proofs a bit.

compiler/backend/bvi_tailrecScript.sml
@@ -1,14 +1,13 @@
 open preamble bviTheory
 open backend_commonTheory;
 
-(* Errors from dummy cases:
-
-   Var 65534                  id_from_op
-   Var 65536                  push_call
-   Var 65537                  mk_tailcall
-*)
-
 val _ = new_theory "bvi_tailrec";
+
+val _ = Define `dummy = bvi$Var 1234567890`;
+
+val MEM_exp_size_imp = Q.store_thm ("MEM_exp_size_imp",
+  `∀xs a. MEM a xs ⇒ bvi$exp_size a < exp2_size xs`,
+  Induct \\ rw [bviTheory.exp_size_def] \\ res_tac \\ fs []);
 
 (* TODO defined in bviSemTheory, should be moved to bviTheory?
    On the other hand: its use here is temporary.
@@ -16,30 +15,36 @@ val _ = new_theory "bvi_tailrec";
 val small_int_def = Define `
   small_int i <=> -268435457 <= i /\ i <= 268435457`;
 
-val MEM_exp_size_imp = Q.store_thm ("MEM_exp_size_imp",
-  `∀xs a. MEM a xs ⇒ bvi$exp_size a < exp2_size xs`,
-  Induct \\ rw [bviTheory.exp_size_def] \\ res_tac \\ fs []);
-
-val args_from_def = Define `
-  (args_from (bvi$Call t (SOME d) as hdl) = SOME (t, d, as, hdl)) ∧
-  (args_from _                            = NONE)
+val is_arith_op_def = Define `
+  is_arith_op Add       = T ∧
+  is_arith_op Mult      = T ∧
+  is_arith_op Sub       = T ∧
+  is_arith_op Div       = T ∧
+  is_arith_op Mod       = T ∧
+  is_arith_op (Const _) = T ∧
+  is_arith_op _         = F
   `;
 
-val is_arithmetic_def = Define `
-  is_arithmetic Add       = T ∧
-  is_arithmetic Mult      = T ∧
-  is_arithmetic Sub       = T ∧
-  is_arithmetic Div       = T ∧
-  is_arithmetic Mod       = T ∧
-  is_arithmetic (Const _) = T ∧
-  is_arithmetic _         = F
+val is_num_rel_def = Define `
+  (is_num_rel LessEq       ⇔ T) ∧
+  (is_num_rel Less         ⇔ T) ∧
+  (is_num_rel Greater      ⇔ T) ∧
+  (is_num_rel GreaterEq    ⇔ T) ∧
+  (is_num_rel (EqualInt _) ⇔ T) ∧
+  (is_num_rel _            ⇔ F)
+  `;
+
+val is_rec_def = Define `
+  (is_rec name (bvi$Call _ d _ NONE) ⇔ d = SOME name) ∧
+  (is_rec _    _                     ⇔ F)
   `;
 
 val _ = Datatype `
   assoc_op = Plus
            | Times
-           | Noop
-  `;
+           | Noop`;
+
+val _ = Datatype `v_ty = Int | Any`;
 
 val to_op_def = Define `
   (to_op Plus  = Add) ∧
@@ -48,16 +53,15 @@ val to_op_def = Define `
   `;
 
 val from_op_def = Define `
-  (from_op Add  = Plus) ∧
-  (from_op Mult = Times) ∧
-  (from_op _    = Noop)
+  from_op op =
+    if op = Add then Plus else
+      if op = Mult then Times else Noop
   `;
 
 val op_eq_def = Define `
-  (op_eq Plus  (Op Add _)  ⇔ T) ∧
-  (op_eq Times (Op Mult _) ⇔ T) ∧
-  (op_eq _     _           ⇔ F)
-  `;
+  (op_eq Plus  (Op op xs) ⇔ op = Add) ∧
+  (op_eq Times (Op op xs) ⇔ op = Mult) ∧
+  (op_eq _     _          ⇔ F)`;
 
 val apply_op_def = Define `
   apply_op op e1 e2 = Op (to_op op) [e1; e2]
@@ -66,7 +70,17 @@ val apply_op_def = Define `
 val id_from_op_def = Define `
   (id_from_op Plus  = bvi$Op (Const 0) []) ∧
   (id_from_op Times = bvi$Op (Const 1) []) ∧
-  (id_from_op Noop  = bvi$Var 65537)
+  (id_from_op Noop  = dummy)
+  `;
+
+val index_of_def = Define `
+  (index_of (bvi$Var i) = SOME i) ∧
+  (index_of _           = NONE)
+  `;
+
+val args_from_def = Define `
+  (args_from (bvi$Call t (SOME d) as hdl) = SOME (t, d, as, hdl)) ∧
+  (args_from _                            = NONE)
   `;
 
 val get_bin_args_def = Define `
@@ -86,34 +100,36 @@ val exp_size_get_bin_args = Q.store_thm ("exp_size_get_bin_args",
   \\ Cases_on `t'` \\ simp [get_bin_args_def]
   \\ fs [bviTheory.exp_size_def]);
 
-(* TODO parametrise on operator *)
-val no_err_def = Define `
-  (no_err (Op (Const i) [])  ⇔ small_int i) ∧
-  (no_err (Op Add [x1; x2])  ⇔ no_err x1 ∧ no_err x2) ∧
-  (no_err (Op Mult [x1; x2]) ⇔ no_err x1 ∧ no_err x2) ∧
-  (no_err _                  ⇔ F)
+val try_update_def = Define `
+  (try_update vty NONE     ts = ts) ∧
+  (try_update vty (SOME n) ts =
+    if n < LENGTH ts
+    then TAKE n ts ++ [vty] ++ DROP (n + 1) ts
+    else ts)
   `;
 
-val is_rec_def = Define `
-  (is_rec name (bvi$Call _ d _ NONE) ⇔ d = SOME name) ∧
-  (is_rec _    _                     ⇔ F)
-  `;
-
-val is_ok_type_def = Define `
-  (is_ok_type (Op op _)    ⇔ is_arithmetic op) ∧
-  (is_ok_type (Let _ x1)   ⇔ is_ok_type x1) ∧
-  (is_ok_type (Tick x1)    ⇔ is_ok_type x1) ∧
-  (is_ok_type (If _ x2 x3) ⇔ is_ok_type x2 ∧ is_ok_type x3) ∧
-  (is_ok_type _            ⇔ F)
-  `;
+(* Allowed expressions `y` in the tail position `f x + y`. *)
+val no_err_def = tDefine "no_err" `
+  (no_err ts (Op op xs) ⇔
+    case op of
+      Const i => small_int i ∧ xs = []
+    | Add     => LENGTH xs = 2 ∧ EVERY (no_err ts) xs
+    | Mult    => LENGTH xs = 2 ∧ EVERY (no_err ts) xs
+    | _       => F) ∧
+  (no_err ts (Var i) ⇔ i < LENGTH ts ∧ EL i ts = Int) ∧
+  (no_err ts _       ⇔ F)`
+  (WF_REL_TAC `measure (exp_size o SND)`
+  \\ Induct
+  \\ rw [bviTheory.exp_size_def]
+  \\ res_tac \\ fs []);
 
 val is_rec_or_rec_binop_def = Define `
-  is_rec_or_rec_binop name op exp ⇔
+  is_rec_or_rec_binop ts name op exp ⇔
     is_rec name exp ∨
     op_eq op exp ∧
       (case get_bin_args exp of
-      | NONE => F
-      | SOME (x1, x2) => is_rec name x1 ∧ no_err x2)
+        NONE        => F
+      | SOME (x, y) => is_rec name x ∧ no_err ts y)
   `;
 
 val assoc_swap_def = Define `
@@ -122,136 +138,193 @@ val assoc_swap_def = Define `
       apply_op op into from
     else
       case get_bin_args into of
-      | NONE => apply_op op into from
-      | SOME (x1, x2) => apply_op op x1 (apply_op op from x2)
+        NONE        => apply_op op into from
+      | SOME (x, y) => apply_op op x (apply_op op from y)
   `;
 
 val rewrite_op_def = tDefine "rewrite_op" `
-  rewrite_op op name exp =
+  rewrite_op ts op loc exp =
     if ¬op_eq op exp then
       (F, exp)
     else
       case get_bin_args exp of
-      | NONE => (F, exp)
+        NONE => (F, exp)
       | SOME (x1, x2) =>
-        let (r1, y1) = rewrite_op op name x1 in
-        let (r2, y2) = rewrite_op op name x2 in
-          case (is_rec_or_rec_binop name op y1,
-                is_rec_or_rec_binop name op y2) of
-          | (F, F) => (F, exp)
-          | (T, T) => (F, exp)
-          | (T, F) => if no_err y2 then (T, assoc_swap op y2 y1) else (F, exp)
-          | (F, T) => if no_err y1 then (T, assoc_swap op y1 y2) else (F, exp)
+        let (r1, y1) = rewrite_op ts op loc x1 in
+        let (r2, y2) = rewrite_op ts op loc x2 in
+          case (is_rec_or_rec_binop ts loc op y1,
+                is_rec_or_rec_binop ts loc op y2) of
+            (T, F) => if no_err ts y2 then (T, assoc_swap op y2 y1) else (F, exp)
+          | (F, T) => if no_err ts y1 then (T, assoc_swap op y1 y2) else (F, exp)
+          | _      => (F, exp)
   `
-  (WF_REL_TAC `measure (exp_size o SND o SND)`
-  \\ rpt strip_tac
-  \\ drule exp_size_get_bin_args
-  \\ fs []);
+  (WF_REL_TAC `measure (exp_size o SND o SND o SND)`
+  \\ rw [exp_size_get_bin_args]);
 
-(* The bool in `(bool * assoc_op) option` tells us if the
-   right-side expression `x2` in `If p x1 x2` returned some
-   assoc_op when `tail_is_ok name x2` was called *)
-val tail_is_ok_def = Define `
-  (tail_is_ok name (Var _)        = NONE) ∧
-  (tail_is_ok name (Let _ x1)     = tail_is_ok name x1) ∧
-  (tail_is_ok name (Tick x1)      = tail_is_ok name x1) ∧
-  (tail_is_ok name (Raise x1)     = NONE) ∧
-  (tail_is_ok name (If _ x2 x3)   =
-    let inl = tail_is_ok name x2 in
-    let inr = tail_is_ok name x3 in
-      (case (inl, inr) of
-        (NONE         , NONE)          => NONE
-      | (SOME (_, iop), NONE)          => SOME (F, iop)
-      | (NONE         , SOME (_, iop)) => SOME (T, iop)
-      | (SOME (_, iop), SOME (_, _))   => SOME (T, iop))) ∧
-  (tail_is_ok name (Call _ _ _ _) = NONE) ∧
-  (tail_is_ok name (Op op xs)     =
-    if op = Add ∨ op = Mult then
-      let iop = from_op op in
-        (case rewrite_op iop name (Op op xs) of
-        | (T, _) => SOME (F, iop)
-        | _ => NONE)
-    else NONE)`;
+val scan_aux_def = tDefine "scan_aux" `
+  (scan_aux ts (If xi xt xe) =
+    let ti = scan_aux ts xi in
+    let tt = scan_aux ti xt in
+    let te = scan_aux ti xe in
+      MAP2 K tt te) ∧
+  (scan_aux ts (Let xs x) =
+    let tt = FOLDL (λt e. Any :: scan_aux t e) ts xs in
+    let t  = scan_aux tt x in
+      DROP (LENGTH xs) t) ∧
+  (scan_aux ts (Tick x) = scan_aux ts x) ∧
+  (scan_aux ts (Op op xs) =
+    if ¬(is_arith_op op ∨ is_num_rel op) then ts
+    else
+      case get_bin_args (Op op xs) of
+        NONE        => ts
+      | SOME (x, y) =>
+          MAP2 (λa b. if a = Int ∨ b = Int then Int else Any)
+            (try_update Int (index_of x) ts)
+            (try_update Int (index_of y) ts)) ∧
+  (scan_aux ts _ = ts)`
+  (WF_REL_TAC `measure (exp_size o SND)`
+  \\ fs [bviTheory.exp_size_def]
+  \\ gen_tac
+  \\ Induct \\ rw []
+  \\ res_tac
+  \\ fs [bviTheory.exp_size_def]);
+
+(* Gather information about expressions:
+
+     - Build context by following order of evaluation during recursion
+       and set variable to Int only if interpretation of the expression would
+       result in Rerr (Rabort Rtype_error) otherwise.
+     - Check if tail positions are arithmetic or variables typed as Int in
+       context.
+     - Check if tail positions carry suitable operation (Add/Mult) and track
+       branch of origin for the operation in conditionals.
+*)
+val scan_expr_def = Define `
+  (scan_expr ts loc (Var n)       = (ts, F, n < LENGTH ts ∧ EL n ts = Int, NONE)) ∧
+  (scan_expr ts loc (If xi xt xe) =
+    let ti = scan_aux ts xi in
+    let (tt, _, pt, ot) = scan_expr ti loc xt in
+    let (te, _, pe, oe) = scan_expr ti loc xe in
+      (MAP2 K tt te, IS_SOME oe, pt ∧ pe,
+       case ot of
+         NONE => oe
+       | _    => ot)) ∧
+  (scan_expr ts loc (Let xs x) =
+    let tt = FOLDL (λt e. Any :: scan_aux t e) ts xs in
+    let (t,_, p, oo) = scan_expr tt loc x in
+      (DROP (LENGTH xs) t, F, p, oo)) ∧
+  (scan_expr ts loc (Raise x) = (ts, F, F, NONE)) ∧
+  (scan_expr ts loc (Tick x) = scan_expr ts loc x) ∧
+  (scan_expr ts loc (Call t d xs h) = (ts, F, F, NONE)) ∧
+  (scan_expr ts loc (Op op xs) =
+    let ok_type = is_arith_op op in
+    let iop =
+      if op = Add ∨ op = Mult then
+        let iop = from_op op in
+          if (FST (rewrite_op ts iop loc (Op op xs)))
+          then SOME iop
+          else NONE
+      else
+        NONE
+      in
+    let tt = scan_aux ts (Op op xs) in
+      (tt, F, ok_type, iop))`
 
 val push_call_def = Define `
   (push_call n op acc exp (SOME (ticks, dest, args, handler)) =
     Call ticks (SOME n) (args ++ [apply_op op exp (Var acc)]) handler) ∧
-  (push_call _ _ _ _ _ = Var 65536) (* dummy *)
+  (push_call _ _ _ _ _ = dummy)
   `;
 
 val mk_tailcall_def = Define `
-  mk_tailcall n op name acc exp =
-    case rewrite_op op name exp of
-    | (F, exp2) => apply_op op exp2 (Var acc)
+  mk_tailcall ts n op name acc exp =
+    case rewrite_op ts op name exp of
+      (F, exp2) => apply_op op exp2 (Var acc)
     | (T, exp2) =>
         (case get_bin_args exp2 of
-        | NONE => Var 65537 (* dummy *)
+          NONE => dummy
         | SOME (call, exp3) =>
           push_call n op acc exp3 (args_from call))
   `;
 
-val rewrite_tail_def = Define `
-  (rewrite_tail n op name acc (Let xs x) =
-    let (r, y) = rewrite_tail n op name (acc + LENGTH xs) x
-    in (r, Let xs y)) ∧
-  (rewrite_tail n op name acc (Tick x) =
-    let (r, y) = rewrite_tail n op name acc x
-    in (r, Tick y)) ∧
-  (rewrite_tail n op name acc (Raise x) = (F, Raise x)) ∧
-  (rewrite_tail n op name acc (If x1 x2 x3) =
-    let (r2, y2) = rewrite_tail n op name acc x2 in
-    let (r3, y3) = rewrite_tail n op name acc x3 in
-    let z2 = if r2 then y2 else apply_op op x2 (Var acc) in
-    let z3 = if r3 then y3 else apply_op op x3 (Var acc) in
-      (r2 ∨ r3, If x1 z2 z3)) ∧
-  (rewrite_tail n op name acc exp =
-    case rewrite_op op name exp of
-      (F, _) => (F, apply_op op exp (Var acc))
-    | (T, exp') =>
-        (case get_bin_args exp' of
-          NONE => (F, apply_op op exp (Var acc))
-        | SOME (call, exp'') =>
-            (T, push_call n op acc exp'' (args_from call))))
-  `;
+(* -------------------------------------------------------------------------- *)
+
+(*val _ = Define `*)
+  (*test_fac = If (Op LessEq [Var 0; Op (Const 1) []])*)
+                (*(Op (Const 1) [])*)
+                (*(Op Mult [Call 0 (SOME 0) [Op Sub [Var 0; Op (Const 1) []]] NONE; Var 0])`*)
+
+(*val _ = Define `*)
+  (*test_foo = If (Op LessEq [Var 0; Var 1])*)
+                (*(Op (Const 1) [])*)
+                (*(Op Mult [Var 0; Var 1])`*)
+
+(*EVAL ``scan_expr [Any] 0 test_fac``*)
+(*EVAL ``scan_expr [Any; Any] 0 test_foo``*)
+(*EVAL ``scan_aux [Any; Any] (Op Add [Var 0; Var 1])``*)
+(*EVAL ``try_update Int (SOME 1) [Any; Any]``*)
+(*EVAL ``try_update Int (SOME 0) [Any; Any]``*)
+
+(* -------------------------------------------------------------------------- *)
+
+(* Unfortunately rewrite_op now requires a context implying some code
+   duplication between rewrite and scan_expr.
+*)
+val rewrite_def = Define `
+  (rewrite (loc, next, op, acc, ts) (If xi xt xe) =
+    let ti = scan_aux ts xi in
+    let (tt, rt, yt) = rewrite (loc, next, op, acc, ti) xt in
+    let (te, re, ye) = rewrite (loc, next, op, acc, ti) xt in
+    let zt = if rt then yt else apply_op op xt (Var acc) in
+    let ze = if re then ye else apply_op op xe (Var acc) in
+      (MAP2 K tt te, rt ∨ re, If xi zt ze)) ∧
+  (rewrite (loc, next, op, acc, ts) (Let xs x) =
+    let tt = FOLDL (λt e. Any :: scan_aux t e) ts xs in
+    let (t, r, y) = rewrite (loc, next, op, acc + LENGTH xs, tt) x in
+      (DROP (LENGTH xs) t, r, Let xs y)) ∧
+  (rewrite (loc, next, op, acc, ts) (Raise x) = (ts, F, Raise x)) ∧
+  (rewrite (loc, next, op, acc, ts) exp =
+    case rewrite_op ts op loc exp of
+      (F, _)    => (ts, F, apply_op op exp (Var acc))
+    | (T, exp1) =>
+      case get_bin_args exp1 of
+        NONE              => (ts, F, apply_op op exp (Var acc))
+      | SOME (call, exp2) =>
+          (ts, T, push_call next op acc exp2 (args_from call)))`;
 
 val check_exp_def = Define `
-  check_exp name exp =
-    if ¬is_ok_type exp then
-      NONE
-    else
-      tail_is_ok name exp
-  `;
+  check_exp loc arity exp =
+    let (_, _, ok, op) = scan_expr (GENLIST (K Any) arity) loc exp in
+      if ¬ok then NONE else op`;
 
 val let_wrap_def = Define `
-  let_wrap num_args id exp =
-    Let ((GENLIST (λi. Var i) num_args) ++ [id]) exp
-  `;
+  let_wrap arity id exp =
+    Let ((GENLIST (λi. Var i) arity) ++ [id]) exp`;
 
 val mk_aux_call_def = Define `
-  mk_aux_call name num_args id =
-    Call 0 (SOME name) (id :: GENLIST (λi. Var (i + 0)) num_args) NONE
-  `;
+  mk_aux_call loc arity id =
+    Call 0 (SOME loc) (id :: GENLIST (λi. Var i) arity) NONE`;
 
 val compile_exp_def = Define `
-  compile_exp n name num_args exp =
-    case check_exp name exp of
-      NONE         => NONE
-    | SOME (_, op) =>
-      let (_, opt) = rewrite_tail n op name num_args exp in
-      let aux = let_wrap num_args (id_from_op op) opt in
-        SOME (aux, opt)
-  `;
+  compile_exp loc next arity exp =
+    case check_exp loc arity exp of
+      NONE    => NONE
+    | SOME op =>
+      let ts          = GENLIST (K Any) arity in
+      let (_, _, opt) = rewrite (loc, next, op, arity, ts) exp in
+      let aux         = let_wrap arity (id_from_op op) opt in
+        SOME (aux, opt)`;
 
 val compile_prog_def = Define `
-  (compile_prog n [] = (n, [])) ∧
-  (compile_prog n ((nm, args, exp)::xs) =
-    case compile_exp n nm args exp of
+  (compile_prog next [] = (next, [])) ∧
+  (compile_prog next ((loc, arity, exp)::xs) =
+    case compile_exp loc next arity exp of
     | NONE =>
-        let (n1, ys) = compile_prog n xs in
-          (n1, (nm, args, exp)::ys)
+        let (n, ys) = compile_prog next xs in
+          (n, (loc, arity, exp)::ys)
     | SOME (exp_aux, exp_opt) =>
-        let (n1, ys) = compile_prog (n + 2) xs in
-        (n1, (nm, args, exp_aux)::(n, args + 1, exp_opt)::ys))
+        let (n, ys) = compile_prog (next + 2) xs in
+        (n, (loc, arity, exp_aux)::(next, arity + 1, exp_opt)::ys))
   `;
 
 val _ = export_theory();
